added embeddings + expanded tauto.

MirrorCharge!/src/ILogicFunc.v
@@ -1,18 +1,19 @@
-Add Rec LoadPath "/Users/jebe/git/Charge/Charge!/bin".
-Add Rec LoadPath "/Users/jebe/git/mirror-core/src/" as MirrorCore.
-Add Rec LoadPath "/Users/jebe/git/mirror-core/coq-ext-lib/theories" as ExtLib.
-
-
-Require Import ILogic ILInsts ZArith.
+Require Import Coq.Bool.Bool ZArith.
+Require Import ILogic ILEmbed.
 Require Import MapPositive.
-Require Import MirrorCore.Ext.ExprCore.
+Require Import ExtLib.Core.RelDec.
+Require Import ExtLib.Data.Positive.
+Require Import ExtLib.Tactics.Consider.
 Require Import MirrorCore.SymI.
 Require Import MirrorCore.Ext.Types.
-Require Import ExtLib.Core.RelDec.
-Require Import Coq.Bool.Bool.
-Require Import ExtLib.Data.Positive.
+Require Import MirrorCore.Ext.ExprCore.
+Require Import MirrorCore.Ext.ExprD.
+
+Set Implicit Arguments.
+Set Strict Implicit.
 
 Inductive ilfunc :=
+| ilf_entails : typ -> ilfunc
 | ilf_true : typ -> ilfunc
 | ilf_false : typ -> ilfunc
 | ilf_and : typ -> ilfunc
@@ -20,31 +21,49 @@ Inductive ilfunc :=
 | ilf_impl : typ -> ilfunc
 | ilf_exists : typ -> typ -> ilfunc
 | ilf_forall : typ -> typ -> ilfunc
+| ilf_embed (from to : typ)
 | fref (fi : positive).
 
-Global Instance RelDec_ilfunc : RelDec (@eq ilfunc) := {
-	rel_dec := fun a b => 
-		match a, b with
-			| ilf_true t, ilf_true t'
-			| ilf_false t, ilf_false t' 
-			| ilf_and t, ilf_and t'
-			| ilf_or t, ilf_or t' 
-			| ilf_impl t, ilf_impl t' => t ?[eq] t'
-			| ilf_forall a t, ilf_forall a' t'
-			| ilf_exists a t, ilf_exists a' t' => a ?[eq] a' && t ?[eq] t'
-			| fref r, fref r' => r ?[eq] r'
-			| _, _ => false
-		end
+Global Instance RelDec_ilfunc : RelDec (@eq ilfunc) :=
+{ rel_dec := fun a b =>
+	       match a, b with
+		 | ilf_entails t, ilf_entails t'
+		 | ilf_true t, ilf_true t'
+		 | ilf_false t, ilf_false t'
+		 | ilf_and t, ilf_and t'
+		 | ilf_or t, ilf_or t'
+		 | ilf_impl t, ilf_impl t' => t ?[eq] t'
+		 | ilf_forall a t, ilf_forall a' t'
+		 | ilf_exists a t, ilf_exists a' t'
+		 | ilf_embed a t, ilf_embed a' t' => a ?[eq] a' && t ?[eq] t'
+		 | fref r, fref r' => r ?[eq] r'
+		 | _, _ => false
+	       end
 }.
 
-Global Instance RelDec_Correct_ilfunc : RelDec_Correct RelDec_ilfunc. admit. Qed.
+Global Instance RelDec_Correct_ilfunc : RelDec_Correct RelDec_ilfunc.
+Proof.
+  constructor.
+  destruct x; destruct y; simpl; intuition; try congruence;
+  repeat match goal with
+           | _ : context [ ?X ?[ eq ] ?Y ] |- _ =>
+             consider (X ?[ eq ] Y); intros; subst
+           | |- context [ ?X ?[ eq ] ?Y ] =>
+             consider (X ?[ eq ] Y); intros; subst
+           | H : _ |- _ =>
+             first [ solve [ inversion H ]
+                   | inversion H; [ clear H; subst ] ]
+         end; intuition.
+Qed.
 
 Section RFunc.
   Variable ts : types.
-  
+
   Definition logic_ops := forall (t : typ),
     option (ILogicOps (typD ts nil t)).
-  
+  Definition embed_ops := forall (t u : typ),
+    option (EmbedOp (typD ts nil t) (typD ts nil u)).
+
   Record function := F
   { ftype : typ
   ; fdenote : typD ts nil ftype
@@ -54,46 +73,44 @@ Section RFunc.
 
   Variable fs : fun_map.
   Variable gs : logic_ops.
- 
-  Local Existing Instance ILFun_Ops.
-  Local Existing Instance ILFun_ILogic.
-
-  Fixpoint gs' (t : typ) : option (ILogicOps (typD ts nil t)):=
-    match t with
-        | tyArr t t' =>
-          match gs' t' with
-            | Some T => Some _
-            | None => None
-          end
-        | t => gs t
-    end.
+  Variable es : embed_ops.
 
   Definition typeof_func (f : ilfunc) : option typ :=
     match f with
       | ilf_true t
       | ilf_false t =>
-        match gs' t with
-   	      | Some _ => Some t
-  	      | None => None
-  	    end
+        match gs t with
+   	  | Some _ => Some t
+  	  | None => None
+  	end
+      | ilf_entails t =>
+        match gs t with
+  	  | Some _ => Some (tyArr t (tyArr t tyProp))
+  	  | None => None
+  	end
       | ilf_and t
       | ilf_or t
       | ilf_impl t =>
-        match gs' t with
-  	      | Some _ => Some (tyArr t (tyArr t t))
-  	      | None => None
-  	    end
-  	  | ilf_forall a t
-  	  | ilf_exists a t =>
-  	  	match gs' t with 
-  	  		| Some _ => Some (tyArr (tyArr a t) t)
-  	  		| None => None
-  	  	end
+        match gs t with
+  	  | Some _ => Some (tyArr t (tyArr t t))
+  	  | None => None
+  	end
+      | ilf_forall a t
+      | ilf_exists a t =>
+  	match gs t with
+  	  | Some _ => Some (tyArr (tyArr a t) t)
+  	  | None => None
+  	end
+      | ilf_embed a b =>
+        match es a b with
+          | None => None
+          | Some _ => Some (tyArr a b)
+        end
       | fref i =>
         match PositiveMap.find i fs with
-  	      | Some f => Some (ftype f)
-  	      | None => None
-  	    end
+  	  | Some f => Some (ftype f)
+  	  | None => None
+  	end
     end.
 
   Definition funcD (f : ilfunc) :
@@ -101,91 +118,130 @@ Section RFunc.
       | Some t => typD ts nil t
       | None => unit
     end.
-    refine (match f as f return match typeof_func f with
-							    | Some t => typD ts nil t
-							    | None => unit
-			                    end 
-			with 
-			| ilf_true t => match gs' t as x return (match match x with
-						                            | Some _ => Some t
-						                            | None => None
-						                            end with
-							| Some t0 => typD ts nil t0
-							| None => unit
-							end) with 
-							| Some t => @ltrue _ t 
-							| None => tt end
-			| ilf_false t => match gs' t as x return (match match x with
-						                            | Some _ => Some t
-						                            | None => None
-						                            end with
-							| Some t0 => typD ts nil t0
-							| None => unit
-							end) with 
-							| Some t => @lfalse _ t 
-							| None => tt end
-			| ilf_and t => match gs' t as x return (match match x with
-						                            | Some _ => Some (tyArr t (tyArr t t))
-						                            | None => None
-						                            end with
-							| Some t0 => typD ts nil t0
-							| None => unit
-							end) with 
-							| Some t => @land _ t 
-							| None => tt end
-			| ilf_impl t => match gs' t as x return (match match x with
-						                            | Some _ => Some (tyArr t (tyArr t t))
-						                            | None => None
-						                            end with
-							| Some t0 => typD ts nil t0
-							| None => unit
-							end) with 
-							| Some t => @limpl _ t 
-							| None => tt end
-			| ilf_or t => match gs' t as x return (match match x with
-						                            | Some _ => Some (tyArr t (tyArr t t))
-						                            | None => None
-						                            end with
-							| Some t0 => typD ts nil t0
-							| None => unit
-							end) with 
-							| Some t => @lor _ t 
-							| None => tt end
-		| fref fi => 
-        match PositiveMap.find fi fs as x
-              return match 
-                match x with
-                  | None => None
-                  | Some f0 => Some f0.(ftype)
+    refine (match f as f
+                  return match typeof_func f with
+			   | Some t => typD ts nil t
+			   | None => unit
+			 end
+	    with
+	      | ilf_true t => match gs t as x
+                                    return (match match x with
+						    | Some _ => Some t
+						    | None => None
+						  end with
+					      | Some t0 => typD ts nil t0
+					      | None => unit
+					    end) with
+				| Some t => @ltrue _ t
+				| None => tt
+                              end
+	      | ilf_false t => match gs t as x
+                                     return (match match x with
+						     | Some _ => Some t
+						     | None => None
+						   end with
+					       | Some t0 => typD ts nil t0
+					       | None => unit
+					     end) with
+				 | Some t => @lfalse _ t
+				 | None => tt
+                               end
+	      | ilf_entails t => match gs t as x
+                                       return (match match x with
+						       | Some _ => Some (tyArr t (tyArr t tyProp))
+						       | None => None
+						     end with
+					         | Some t0 => typD ts nil t0
+					         | None => unit
+					       end) with
+			           | Some t => @lentails _ t
+			           | None => tt
+                             end
+	      | ilf_and t => match gs t as x
+                                   return (match match x with
+						   | Some _ => Some (tyArr t (tyArr t t))
+						   | None => None
+						 end with
+					     | Some t0 => typD ts nil t0
+					     | None => unit
+					   end) with
+			       | Some t => @land _ t
+			       | None => tt
+                             end
+
+	      | ilf_impl t => match gs t as x
+                                    return (match match x with
+						    | Some _ => Some (tyArr t (tyArr t t))
+						    | None => None
+						  end with
+					      | Some t0 => typD ts nil t0
+					      | None => unit
+					    end) with
+				| Some t => @limpl _ t
+				| None => tt
+                              end
+	      | ilf_or t => match gs t as x
+                                  return (match match x with
+						  | Some _ => Some (tyArr t (tyArr t t))
+						  | None => None
+						end with
+					    | Some t0 => typD ts nil t0
+					    | None => unit
+					  end) with
+			      | Some t => @lor _ t
+			      | None => tt
+                            end
+	      | fref fi =>
+                match PositiveMap.find fi fs as x
+                      return match
+                        match x with
+                          | None => None
+                          | Some f0 => Some f0.(ftype)
+                        end
+                      with
+                        | None => unit
+                        | Some t => typD ts nil t
+                      end
+                with
+                  | None => tt
+                  | Some f => f.(fdenote)
                 end
-              with
-                | None => unit
-                | Some t => typD ts nil t
-              end
-        with
-          | None => tt
-          | Some f => f.(fdenote)
-        end		
-        | ilf_exists a t => match gs' t as x return (match match x with
-						                            | Some _ => Some (tyArr (tyArr a t) t)
-						                            | None => None
-						                            end with
-							| Some t0 => typD ts nil t0
-							| None => unit
-							end) with 
-							| Some t0 => @lexists _ t0 (typD ts nil a)
-							| None => tt end	
-         | ilf_forall a t => match gs' t as x return (match match x with
-						                            | Some _ => Some (tyArr (tyArr a t) t)
-						                            | None => None
-						                            end with
-							| Some t0 => typD ts nil t0
-							| None => unit
-							end) with 
-							| Some t0 => @lforall _ t0 (typD ts nil a)
-							| None => tt end end).	
-Defined.
-Print RSym.
+              | ilf_exists a t => match gs t as x return (match match x with
+						                  | Some _ => Some (tyArr (tyArr a t) t)
+						                  | None => None
+						                end with
+							    | Some t0 => typD ts nil t0
+							    | None => unit
+							  end) with
+				    | Some t0 => @lexists _ t0 (typD ts nil a)
+				    | None => tt
+                                  end
+              | ilf_forall a t => match gs t as x return (match match x with
+						                  | Some _ => Some (tyArr (tyArr a t) t)
+						                  | None => None
+						                end with
+							    | Some t0 => typD ts nil t0
+							    | None => unit
+							  end) with
+				    | Some t0 => @lforall _ t0 (typD ts nil a)
+				    | None => tt
+                                  end
+              | ilf_embed t u =>
+                match es t u as x
+                      return match match x with
+				     | Some _ => Some (tyArr t u)
+				     | None => None
+				   end with
+			       | Some t0 => typD ts nil t0
+			       | None => unit
+			     end
+                with
+		  | Some t0 => @embed _ _ t0
+		  | None => tt
+                end
+            end).
+  Defined.
+
   Global Instance RSym_ilfunc : RSym (@typD ts) ilfunc :=
   { typeof_sym := typeof_func
   ; sym_eqb := fun a b => Some (rel_dec a b)
@@ -193,21 +249,38 @@ Print RSym.
   }.
 End RFunc.
 
-
 Section demo.
-  Context {T : Type} {ILO : ILogicOps T}.
+  Context {T} `{ILT : ILogicOps T}.
+  Context {U} `{ILU : ILogicOps U}.
+  Context {T_U_embed : EmbedOp T U}.
 
-  Definition ts : types := (default_type T)::(default_type nat)::nil.
+  Definition ts : types := (default_type T)::(default_type U)::(default_type nat)::nil.
 
   Definition logics : logic_ops ts :=
     fun t => match t with
-             | tyType 0 => Some ILO
-             | _ => None
+               | tyType 0 => Some ILT
+               | tyType 1 => Some ILU
+               | tyProp => Some _
+               | _ => None
              end.
 
-  Axiom eq_nat : nat -> nat -> T.
-  
-  Definition eq_nat_emb := F ts (tyArr (tyType 1) (tyArr (tyType 1) (tyType 0))) (eq_nat).
+  Definition embeds : embed_ops ts :=
+    fun t u =>
+      match t , u with
+        | tyProp , tyProp => Some {| embed := fun x => x |}
+        | tyType 0 , tyType 0 => Some {| embed := fun x => x |}
+        | tyType 1 , tyType 1 => Some {| embed := fun x => x |}
+        | tyType 0 , tyType 1 => Some _
+        | _ , _ => None
+      end.
+
+  Variable eq_nat : nat -> nat -> T.
+
+  Let T_T := tyType 0.
+  Let T_U := tyType 1.
+  Let T_nat := tyType 2.
+
+  Definition eq_nat_emb := F ts (tyArr T_nat (tyArr T_nat (tyType 0))) (eq_nat).
 
   Definition funcs : fun_map ts := PositiveMap.add (1%positive) (eq_nat_emb) (PositiveMap.empty _).
 
@@ -216,18 +289,16 @@ Section demo.
   Definition inj_impl (p q : expr ilfunc) : expr ilfunc := App (App (Inj (ilf_impl (tyType 0))) p) q.
   Definition inj_true : expr ilfunc := Inj (ilf_true (tyType 0)).
   Definition inj_false : expr ilfunc := Inj (ilf_false (tyType 0)).
-  Definition inj_exists (a : typ) (f : expr ilfunc) : expr ilfunc := 
+  Definition inj_exists (a : typ) (f : expr ilfunc) : expr ilfunc :=
   	App (Inj (ilf_exists a (tyType 0))) (Abs a f).
-  Definition inj_forall (a : typ) (f : expr ilfunc) : expr ilfunc := 
+  Definition inj_forall (a : typ) (f : expr ilfunc) : expr ilfunc :=
   	App (Inj (ilf_forall a (tyType 0))) (Abs a f).
   Definition inj_eq_nat (a b : expr ilfunc) : expr ilfunc :=
     App (App (Inj (fref (1%positive))) a) b.
 
-
-
   Definition tm : expr ilfunc := inj_and inj_true inj_true.
-  Definition tm2 : expr ilfunc := inj_forall (tyType 1) (inj_eq_nat (Var 0) (Var 0)).
-  Require Import MirrorCore.Ext.ExprD.
+  Definition tm2 : expr ilfunc := inj_forall T_nat (inj_eq_nat (Var 0) (Var 0)).
+
 
   (** TODO: Here we run into a problem because the [expr] type is
    ** fixed to the [typ] defined in [MirrorCore.Ext.Types].
@@ -235,7 +306,26 @@ Section demo.
    **   types.
    **)
 
-  Eval cbv beta iota zeta delta - [ltrue land] in @exprD ts _ (RSym_ilfunc ts funcs logics) nil nil tm (tyType 0).
-  Eval cbv beta iota zeta delta - [ltrue land lforall] in @exprD ts _ (RSym_ilfunc ts funcs logics) nil nil tm2 (tyType 0).
+  Definition testD := @exprD ts _ (@RSym_ilfunc ts funcs logics embeds) nil nil.
+
+  Eval cbv beta iota zeta delta - [ltrue land] in testD tm (tyType 0).
+  Eval cbv beta iota zeta delta - [ltrue land lforall] in testD tm2 (tyType 0).
 
 End demo.
+
+(*
+Section enhanced_resolution.
+
+  Local Existing Instance ILFun_Ops.
+  Local Existing Instance ILFun_ILogic.
+
+  Fixpoint gs' (t : typ) : option (ILogicOps (typD ts nil t)):=
+    match t with
+      | tyArr t t' =>
+        match gs' t' with
+          | Some T => Some _
+          | None => None
+        end
+      | t => gs t
+    end.
+*)
